pulse/examples/dsls/mini_steel/Pulse.Soundness.STEquiv.fst
@@ -26,23 +26,23 @@ let abs_and_app0 (ty:R.term) (b:R.term) =
 
 
 // x:ty -> vprop_equiv p q ~ x:ty -> vprop_equiv ((fun y -> p) x) ((fun y -> q) x)
-let stt_vprop_equiv_abstract (#f:stt_env) (#g:env) (#post0 #post1:pure_term) (#pf:_) (#ty:_)
+let stt_vprop_equiv_abstract (#f:stt_env) (#g:env) (#post0 #post1:term) (#pf:_) (#ty:_)
                              (d:RT.typing (extend_env_l f g) pf 
                                           (mk_arrow (ty, R.Q_Explicit)
-                                                    (stt_vprop_equiv (elab_pure post0) (elab_pure post1))))
+                                                    (stt_vprop_equiv (elab_term post0) (elab_term post1))))
   : GTot (RT.typing (extend_env_l f g) pf
                     (mk_arrow (ty, R.Q_Explicit)
-                              (stt_vprop_equiv (abs_and_app0 ty (elab_pure post0))
-                                               (abs_and_app0 ty (elab_pure post1)))))
+                              (stt_vprop_equiv (abs_and_app0 ty (elab_term post0))
+                                               (abs_and_app0 ty (elab_term post1)))))
   = admit()
 
 let inst_intro_vprop_post_equiv (#g:R.env) (#ty:R.term) (#u:_)
                                 (d_ty:RT.typing g ty (RT.tm_type u))
                                 (#post0 #post1:R.term)
                                 (d_0:RT.typing g post0 
-                                                (mk_arrow (ty, R.Q_Explicit) (elab_pure Tm_VProp)))
+                                                (mk_arrow (ty, R.Q_Explicit) (elab_term Tm_VProp)))
                                 (d_1:RT.typing g post1 
-                                                (mk_arrow (ty, R.Q_Explicit) (elab_pure Tm_VProp)))
+                                                (mk_arrow (ty, R.Q_Explicit) (elab_term Tm_VProp)))
                                 (#pf:_)
                                 (eq:RT.typing g pf (mk_arrow (ty, R.Q_Explicit) 
                                                              (stt_vprop_equiv (app0 post0) (app0 post1))))
@@ -55,25 +55,25 @@ let stt_vprop_post_equiv_is_prop (#g:R.env) (#ty:R.term) (#u:_)
                                  (d_ty:RT.typing g ty (RT.tm_type u))
                                  (#post0 #post1:R.term)
                                  (d_0:RT.typing g post0 
-                                                (mk_arrow (ty, R.Q_Explicit) (elab_pure Tm_VProp)))
+                                                (mk_arrow (ty, R.Q_Explicit) (elab_term Tm_VProp)))
                                  (d_1:RT.typing g post1 
-                                                (mk_arrow (ty, R.Q_Explicit) (elab_pure Tm_VProp)))
+                                                (mk_arrow (ty, R.Q_Explicit) (elab_term Tm_VProp)))
   : GTot (RT.typing g (stt_vprop_post_equiv u ty post0 post1) RT.tm_prop)
   = admit()
 
 let inst_sub_stt (#g:R.env) (#u:_) (#a #pre1 #pre2 #post1 #post2 #r:R.term)
                  (d_a: RT.typing g a (RT.tm_type u))
-                 (d_pre1: RT.typing g pre1 (elab_pure Tm_VProp))
-                 (d_pre2: RT.typing g pre2 (elab_pure Tm_VProp))
-                 (d_post1:RT.typing g post1 (mk_arrow (a, R.Q_Explicit) (elab_pure Tm_VProp)))
-                 (d_post2:RT.typing g post2 (mk_arrow (a, R.Q_Explicit) (elab_pure Tm_VProp)))
+                 (d_pre1: RT.typing g pre1 (elab_term Tm_VProp))
+                 (d_pre2: RT.typing g pre2 (elab_term Tm_VProp))
+                 (d_post1:RT.typing g post1 (mk_arrow (a, R.Q_Explicit) (elab_term Tm_VProp)))
+                 (d_post2:RT.typing g post2 (mk_arrow (a, R.Q_Explicit) (elab_term Tm_VProp)))
                  (pre_equiv:RT.typing g (`()) (stt_vprop_equiv pre1 pre2))
                  (post_equiv:RT.typing g (`()) (stt_vprop_post_equiv u a post1 post2))
                  (d_r:RT.typing g r (mk_stt_comp u a pre1 post1))
   : GTot (RT.typing g (mk_sub_stt u a pre1 pre2 post1 post2 r) (mk_stt_comp u a pre2 post2))
   = admit()
 
-let vprop_arrow (t:pure_term) : pure_term = Tm_Arrow (null_binder t) None (C_Tot Tm_VProp)
+let vprop_arrow (t:term) : term = Tm_Arrow (null_binder t) None (C_Tot Tm_VProp)
 
 #push-options "--fuel 2 --ifuel 1 --z3rlimit_factor 4 --query_stats"
 let st_equiv_soundness (f:stt_env)
@@ -81,14 +81,14 @@ let st_equiv_soundness (f:stt_env)
                        (c0 c1:ln_comp) 
                        (d:st_equiv f g c0 c1)
                        (r:R.term)
-                       (d_r:RT.typing (extend_env_l f g) r (elab_pure_comp c0)) 
-  : GTot (RT.typing (extend_env_l f g) (elab_sub c0 c1 r) (elab_pure_comp c1))
+                       (d_r:RT.typing (extend_env_l f g) r (elab_comp c0)) 
+  : GTot (RT.typing (extend_env_l f g) (elab_sub c0 c1 r) (elab_comp c1))
   = if C_ST? c0 && C_ST? c1 then
     let ST_VPropEquiv _ _ _ x pre_typing res_typing post_typing eq_pre eq_post = d in
     // assert (None? (lookup_ty g x));
     assert (None? (lookup g x));
-    assume (~(x `Set.mem` RT.freevars (elab_pure (comp_post c0))));
-    assume (~(x `Set.mem` RT.freevars (elab_pure (comp_post c1))));      
+    assume (~(x `Set.mem` RT.freevars (elab_term (comp_post c0))));
+    assume (~(x `Set.mem` RT.freevars (elab_term (comp_post c1))));      
     let open_term_spec (e:R.term) (x:var)
         : Lemma 
           (RT.open_term e x == RT.open_or_close_term' e (RT.open_with_var x) 0)
@@ -100,22 +100,22 @@ let st_equiv_soundness (f:stt_env)
     elab_open_commute (comp_post c0) x;
     elab_open_commute (comp_post c1) x;      
     let post_equiv
-      : RT.typing (RT.extend_env (extend_env_l f g) x (elab_pure (comp_res c0)))
+      : RT.typing (RT.extend_env (extend_env_l f g) x (elab_term (comp_res c0)))
                   (`())
                   (stt_vprop_equiv 
-                    (RT.open_term (elab_pure (comp_post c0)) x)
-                    (RT.open_term (elab_pure (comp_post c1)) x))
+                    (RT.open_term (elab_term (comp_post c0)) x)
+                    (RT.open_term (elab_term (comp_post c1)) x))
         = VPropEquiv.vprop_equiv_unit_soundness post_typing eq_post
     in
-    let t0 = elab_pure (comp_res c0)  in
+    let t0 = elab_term (comp_res c0)  in
     let r_res_typing = tot_typing_soundness res_typing in
-    RT.close_open_inverse (elab_pure (comp_post c0)) x;
-    RT.close_open_inverse (elab_pure (comp_post c1)) x;      
+    RT.close_open_inverse (elab_term (comp_post c0)) x;
+    RT.close_open_inverse (elab_term (comp_post c1)) x;      
     let d 
       : RT.typing (extend_env_l f g) _ 
                   (mk_arrow (t0, R.Q_Explicit)
-                            (stt_vprop_equiv (elab_pure (comp_post c0))
-                                             (elab_pure (comp_post c1))))
+                            (stt_vprop_equiv (elab_term (comp_post c0))
+                                             (elab_term (comp_post c1))))
         = RT.T_Abs _ _ _ (`()) _ _ _ R.Q_Explicit
                  r_res_typing
                  post_equiv
@@ -124,13 +124,13 @@ let st_equiv_soundness (f:stt_env)
     let abs_post0_typing
       : RT.typing (extend_env_l f g)
                   (elab_comp_post c0) // mk_abs t0 (elab_pure (comp_post c0)))
-                  (elab_pure (vprop_arrow (comp_res c0)))
+                  (elab_term (vprop_arrow (comp_res c0)))
       = mk_t_abs_tot _ _ _ res_typing post_typing
     in
     let abs_post1_typing
       : RT.typing (extend_env_l f g)
                   (elab_comp_post c1) //mk_abs t0 (elab_pure (comp_post c1)))
-                  (elab_pure (vprop_arrow (comp_res c0)))
+                  (elab_term (vprop_arrow (comp_res c0)))
       = mk_t_abs_tot _ _ _ res_typing (fst (vprop_equiv_typing _ _ _ _ eq_post) post_typing)
     in
     let (| pf, d |) =
