pulse/examples/dsls/mini_steel/Pulse.Soundness.fst
@@ -26,40 +26,40 @@ module EPure = Pulse.Elaborate.Pure
 let soundness_t (d:'a) = 
     f:stt_env ->
     g:env ->
-    t:term ->
-    c:pure_comp ->
-    d':src_typing f g t c{d' << d} ->
+    t:st_term ->
+    c:comp ->
+    d':st_typing f g t c{d' << d} ->
     GTot (RT.typing (extend_env_l f g)
-                    (elab_src_typing d')
-                    (elab_pure_comp c))
+                    (elab_st_typing d')
+                    (elab_comp c))
 
 let tabs_t (d:'a) = 
     #f:stt_env ->
     #g:env ->
     #u:universe ->
-    #ty:pure_term ->
+    #ty:term ->
     q:option qualifier ->
     ppname:ppname ->
     t_typing:tot_typing f g ty (Tm_Type u) { t_typing << d } ->
-    #body:term ->
-    #x:var { None? (lookup g x) /\ ~(x `Set.mem` freevars body) } ->
-    #c:pure_comp ->
-    body_typing:src_typing f ((x, Inl ty)::g) (open_term body x) c { body_typing << d } ->
+    #body:st_term ->
+    #x:var { None? (lookup g x) /\ ~(x `Set.mem` freevars_st body) } ->
+    #c:comp ->
+    body_typing:st_typing f ((x, Inl ty)::g) (open_st_term body x) c { body_typing << d } ->
     GTot (RT.typing (extend_env_l f g)
-                    (mk_abs_with_name ppname (elab_pure ty) (elab_qual q) (RT.close_term (elab_src_typing body_typing) x))
-                      (elab_pure (Tm_Arrow {binder_ty=ty;binder_ppname=ppname} q (close_pure_comp c x))))
+                    (mk_abs_with_name ppname (elab_term ty) (elab_qual q) (RT.close_term (elab_st_typing body_typing) x))
+                      (elab_term (Tm_Arrow {binder_ty=ty;binder_ppname=ppname} q (close_comp c x))))
 
 let lift_soundness
   (f:stt_env)
   (g:env)
-  (t:term)
-  (c:pure_comp)
-  (d:src_typing f g t c{T_Lift? d})
+  (t:st_term)
+  (c:comp)
+  (d:st_typing f g t c{T_Lift? d})
   (soundness:soundness_t d)
-  : GTot (RT.typing (extend_env_l f g) (elab_src_typing d) (elab_pure_comp c)) =
-  LN.src_typing_ln d;
+  : GTot (RT.typing (extend_env_l f g) (elab_st_typing d) (elab_comp c)) =
+  LN.st_typing_ln d;
   let T_Lift _ e c1 c2 e_typing lc = d in
-  LN.src_typing_ln e_typing;
+  LN.st_typing_ln e_typing;
   match lc with
   | Lift_STAtomic_ST _ _ ->
     Lift.elab_lift_stt_atomic_typing f g
@@ -68,59 +68,57 @@ let lift_soundness
     let (| reveal_a, reveal_a_typing |) = w in
     Lift.elab_lift_stt_ghost_typing f g
       c1 c2 _ (soundness _ _ _ _ e_typing) lc
-      _ (soundness _ _ _ _ reveal_a_typing)
+      _ (tot_typing_soundness reveal_a_typing)
 
 let frame_soundness
   (f:stt_env)
   (g:env)
-  (t:term)
-  (c:pure_comp)
-  (d:src_typing f g t c{T_Frame? d})
+  (t:st_term)
+  (c:comp)
+  (d:st_typing f g t c{T_Frame? d})
   (soundness:soundness_t d)
-  : GTot (RT.typing (extend_env_l f g) (elab_src_typing d) (elab_pure_comp c)) =
+  : GTot (RT.typing (extend_env_l f g) (elab_st_typing d) (elab_comp c)) =
 
   let T_Frame _ e c frame frame_typing e_typing = d in
   let r_e_typing = soundness _ _ _ _ e_typing in
-  LN.src_typing_ln e_typing;
+  LN.st_typing_ln e_typing;
   Frame.elab_frame_typing f g _ _ frame frame_typing r_e_typing
 
 let stapp_soundness
   (f:stt_env)
   (g:env)
-  (t:term)
-  (c:pure_comp)
-  (d:src_typing f g t c{T_STApp? d})
+  (t:st_term)
+  (c:comp)
+  (d:st_typing f g t c{T_STApp? d})
   (soundness:soundness_t d)
-  : GTot (RT.typing (extend_env_l f g) (elab_src_typing d) (elab_pure_comp c)) =
+  : GTot (RT.typing (extend_env_l f g) (elab_st_typing d) (elab_comp c)) =
 
-  let T_STApp _ head ppname formal q res arg head_typing arg_typing = d in
-  let E arg_typing = arg_typing in
-  let r_head = elab_src_typing head_typing in
-  let r_arg = elab_pure arg in
-  elab_pure_equiv arg_typing;
+  let T_STApp _ head formal q res arg head_typing arg_typing = d in
+  let r_head = elab_term head in
+  let r_arg = elab_term arg in
   let r_head_typing
-    : RT.typing _ r_head (elab_pure (Tm_Arrow {binder_ty=formal;binder_ppname=ppname} q res))
-    = soundness _ _ _ _ head_typing
+    : RT.typing _ r_head (elab_term (Tm_Arrow {binder_ty=formal;binder_ppname=RT.pp_name_default} q res))
+    = tot_typing_soundness head_typing
   in
-  let r_arg_typing = soundness _ _ _ _ arg_typing in
+  let r_arg_typing = tot_typing_soundness arg_typing in
   elab_comp_open_commute res arg;
-  RT.T_App _ _ _ (binder_of_t_q_s (elab_pure formal) (elab_qual q) ppname)
-                 (elab_pure_comp res)
+  RT.T_App _ _ _ (binder_of_t_q_s (elab_term formal) (elab_qual q) RT.pp_name_default)
+                 (elab_comp res)
                  r_head_typing
                  r_arg_typing
 
 let stequiv_soundness
   (f:stt_env)
   (g:env)
-  (t:term)
-  (c:pure_comp)
-  (d:src_typing f g t c{T_Equiv? d})
+  (t:st_term)
+  (c:comp)
+  (d:st_typing f g t c{T_Equiv? d})
   (soundness:soundness_t d)            
-  : GTot (RT.typing (extend_env_l f g) (elab_src_typing d) (elab_pure_comp c)) =
+  : GTot (RT.typing (extend_env_l f g) (elab_st_typing d) (elab_comp c)) =
 
   let T_Equiv _ e c c' e_typing equiv = d in
-  LN.src_typing_ln d;
-  LN.src_typing_ln e_typing;
+  LN.st_typing_ln d;
+  LN.st_typing_ln e_typing;
   let r_e_typing = soundness _ _ _ _ e_typing in 
   STEquiv.st_equiv_soundness _ _ _ _ equiv _ r_e_typing
 
@@ -130,24 +128,24 @@ let stequiv_soundness
 let bind_soundness
   (#f:stt_env)
   (#g:env)
-  (#t:term)
-  (#c:pure_comp)
-  (d:src_typing f g t c{T_Bind? d})
+  (#t:st_term)
+  (#c:comp)
+  (d:st_typing f g t c{T_Bind? d})
   (soundness: soundness_t d)
   (mk_t_abs: tabs_t d)
   : GTot (RT.typing (extend_env_l f g)
-                    (elab_src_typing d)
-                    (elab_pure_comp c))
+                    (elab_st_typing d)
+                    (elab_comp c))
   = let T_Bind _ e1 e2 c1 c2 x c e1_typing t_typing e2_typing bc = d in
-    LN.src_typing_ln e1_typing;
-    LN.src_typing_ln e2_typing;      
-    FV.src_typing_freevars_inv e1_typing x;
+    LN.st_typing_ln e1_typing;
+    LN.st_typing_ln e2_typing;      
+    FV.st_typing_freevars_inv e1_typing x;
     let r1_typing
-      : RT.typing _ _ (elab_pure_comp c1)
+      : RT.typing _ _ (elab_comp c1)
       = soundness _ _ _ _ e1_typing
     in
     let r2_typing
-      : RT.typing _ _ (elab_pure (Tm_Arrow (null_binder (comp_res c1)) None (close_pure_comp c2 x)))
+      : RT.typing _ _ (elab_term (Tm_Arrow (null_binder (comp_res c1)) None (close_comp c2 x)))
       = mk_t_abs None _ t_typing e2_typing
     in
     match bc with
@@ -161,33 +159,33 @@ let bind_soundness
            _ r2_typing bc
            (tot_typing_soundness t2_typing)
            (mk_t_abs_tot _ _ _ t2_typing post2_typing)
-           (elab_pure reveal_a)
-           (soundness _ _ _ _ reveal_a_typing)
+           (elab_term reveal_a)
+           (tot_typing_soundness reveal_a_typing)
     | Bind_comp_ghost_r _ _ _ _ (| reveal_b, reveal_b_typing |) t2_typing y post2_typing ->
          Bind.elab_bind_ghost_r_typing f g _ _ _ x _ r1_typing
            _ r2_typing bc
            (tot_typing_soundness t2_typing)
            (mk_t_abs_tot _ _ _ t2_typing post2_typing)
-           (elab_pure reveal_b)
-           (soundness _ _ _ _ reveal_b_typing)
+           (elab_term reveal_b)
+           (tot_typing_soundness reveal_b_typing)
 #pop-options
 
 let intro_exists_soundness
   (#f:stt_env)
   (#g:env)
-  (#t:term)
-  (#c:pure_comp)
-  (d:src_typing f g t c{T_IntroExists? d})
+  (#t:st_term)
+  (#c:comp)
+  (d:st_typing f g t c{T_IntroExists? d})
   : GTot (RT.typing (extend_env_l f g)
-                    (elab_src_typing d)
-                    (elab_pure_comp c)) =
+                    (elab_st_typing d)
+                    (elab_comp c)) =
 
   let t0 = t in
   let T_IntroExists _ u t p e t_typing p_typing e_typing = d in
   let ru = elab_universe u in
-  let rt = elab_pure t in
-  let rp = elab_pure p in
-  let re = elab_pure e in
+  let rt = elab_term t in
+  let rp = elab_term p in
+  let re = elab_term e in
 
   let rt_typing : RT.typing _ rt (R.pack_ln (R.Tv_Type ru)) =
     tot_typing_soundness t_typing in
@@ -209,7 +207,7 @@ let intro_exists_soundness
           RT.open_or_close_term' rp (RT.OpenWith re) 0);
 
   elab_open_commute' p e 0;
-  assert (elab_pure (open_term' p e 0) ==
+  assert (elab_term (open_term' p e 0) ==
           R.pack_ln (R.Tv_App (mk_abs rt R.Q_Explicit rp) (re, R.Q_Explicit)));
 
   Exists.intro_exists_soundness rt_typing rp_typing re_typing
@@ -223,42 +221,42 @@ assume val freevars_not_mem_close (t:R.term) (x:var) (i:nat)
 let elim_exists_soundness
   (#f:stt_env)
   (#g:env)
-  (#t:term)
-  (#c:pure_comp)
-  (d:src_typing f g t c{T_ElimExists? d})
+  (#t:st_term)
+  (#c:comp)
+  (d:st_typing f g t c{T_ElimExists? d})
   : GTot (RT.typing (extend_env_l f g)
-                    (elab_src_typing d)
-                    (elab_pure_comp c)) =
+                    (elab_st_typing d)
+                    (elab_comp c)) =
 
   let T_ElimExists _ u t p x t_typing p_typing = d in
   let ru = elab_universe u in
-  let rt = elab_pure t in
-  let rp = elab_pure p in
+  let rt = elab_term t in
+  let rp = elab_term p in
   let rt_typing = tot_typing_soundness t_typing in
   let rp_typing
     : RT.typing (extend_env_l f g)
-                (mk_exists ru (elab_pure t)
-                   (mk_abs (elab_pure t) R.Q_Explicit (elab_pure p)))
+                (mk_exists ru (elab_term t)
+                   (mk_abs (elab_term t) R.Q_Explicit (elab_term p)))
                 vprop_tm
     = tot_typing_soundness p_typing in
   let rp_typing = Exists.exists_inversion rp_typing in
 
-  FV.src_typing_freevars_inv d x;
+  FV.st_typing_freevars_inv d x;
   assert (~ (Set.mem x (freevars t)));
   assert (~ (Set.mem x (freevars p)));
 
   let x_tm = Tm_Var {nm_index=x;nm_ppname=RT.pp_name_default} in
   let rx_tm = R.pack_ln (R.Tv_Var (R.pack_bv (RT.make_bv x tun))) in
   let rx_bv = R.pack_ln (R.Tv_BVar (R.pack_bv (RT.make_bv 0 tun))) in
-  assert (elab_pure (mk_reveal u t x_tm) ==
+  assert (elab_term (mk_reveal u t x_tm) ==
           EPure.mk_reveal ru rt rx_tm);
   calc (==) {
-    elab_pure (close_term' (open_term' p (mk_reveal u t x_tm) 0) x 0);
+    elab_term (close_term' (open_term' p (mk_reveal u t x_tm) 0) x 0);
        (==) { elab_close_commute'
                 (open_term' p (mk_reveal u t x_tm) 0)
                 x
                 0 }
-    RT.open_or_close_term' (elab_pure (open_term' p (mk_reveal u t x_tm) 0)) (RT.CloseVar x) 0;
+    RT.open_or_close_term' (elab_term (open_term' p (mk_reveal u t x_tm) 0)) (RT.CloseVar x) 0;
        (==) { elab_open_commute'
                 p
                 (mk_reveal u t x_tm)
@@ -287,16 +285,16 @@ let elim_exists_soundness
 let while_soundness
   (#f:stt_env)
   (#g:env)
-  (#t:term)
-  (#c:pure_comp)
-  (d:src_typing f g t c{T_While? d})
+  (#t:st_term)
+  (#c:comp)
+  (d:st_typing f g t c{T_While? d})
   (soundness: soundness_t d)
   : GTot (RT.typing (extend_env_l f g)
-                    (elab_src_typing d)
-                    (elab_pure_comp c)) =
+                    (elab_st_typing d)
+                    (elab_comp c)) =
 
   let T_While _ inv cond body inv_typing cond_typing body_typing = d in
-  let rinv = mk_abs bool_tm R.Q_Explicit (elab_pure inv) in
+  let rinv = mk_abs bool_tm R.Q_Explicit (elab_term inv) in
   let rinv_typing
     : RT.typing _
         (mk_exists uzero bool_tm rinv)
@@ -308,24 +306,24 @@ let while_soundness
         (mk_arrow (bool_tm, R.Q_Explicit) vprop_tm) =
     Exists.exists_inversion rinv_typing in
   let rcond_typing
-    : RT.typing _ (elab_src_typing cond_typing)
+    : RT.typing _ (elab_st_typing cond_typing)
         (mk_stt_comp uzero bool_tm (mk_exists uzero bool_tm rinv) rinv) =
     soundness f g cond (comp_while_cond inv) cond_typing in
 
   elab_open_commute' inv tm_true 0;
-  assume (R.pack_ln (R.Tv_App (mk_abs bool_tm R.Q_Explicit (elab_pure inv)) (true_tm, R.Q_Explicit)) ==
-          RT.open_or_close_term' (elab_pure inv) (RT.OpenWith true_tm) 0);
+  assume (R.pack_ln (R.Tv_App (mk_abs bool_tm R.Q_Explicit (elab_term inv)) (true_tm, R.Q_Explicit)) ==
+          RT.open_or_close_term' (elab_term inv) (RT.OpenWith true_tm) 0);
 
   let rbody_typing
-    : RT.typing _ (elab_src_typing body_typing)
+    : RT.typing _ (elab_st_typing body_typing)
         (mk_stt_comp uzero unit_tm
            (R.pack_ln (R.Tv_App rinv (true_tm, R.Q_Explicit)))
            (mk_abs unit_tm R.Q_Explicit (mk_exists uzero bool_tm rinv))) =
     soundness f g body (comp_while_body inv) body_typing in
 
   elab_open_commute' inv tm_false 0;
-  assume (R.pack_ln (R.Tv_App (mk_abs bool_tm R.Q_Explicit (elab_pure inv)) (false_tm, R.Q_Explicit)) ==
-          RT.open_or_close_term' (elab_pure inv) (RT.OpenWith false_tm) 0);
+  assume (R.pack_ln (R.Tv_App (mk_abs bool_tm R.Q_Explicit (elab_term inv)) (false_tm, R.Q_Explicit)) ==
+          RT.open_or_close_term' (elab_term inv) (RT.OpenWith false_tm) 0);
 
   While.while_soundness rinv_typing rcond_typing rbody_typing
 
@@ -334,22 +332,22 @@ let while_soundness
 let if_soundness
   (f:stt_env)
   (g:env)
-  (t:term)
-  (c:pure_comp)
-  (d:src_typing f g t c{T_If? d})
+  (t:st_term)
+  (c:comp)
+  (d:st_typing f g t c{T_If? d})
   (soundness:soundness_t d)
-  (ct_soundness: (f:stt_env -> g:env -> c:pure_comp -> uc:universe ->
+  (ct_soundness: (f:stt_env -> g:env -> c:comp -> uc:universe ->
                   d':comp_typing f g c uc{d' << d} ->
               GTot (RT.typing (extend_env_l f g)
-                              (elab_pure_comp c)
+                              (elab_comp c)
                               (RT.tm_type (elab_universe uc)))))
   : GTot (RT.typing (extend_env_l f g)
-                    (elab_src_typing d)
-                    (elab_pure_comp c)) =
+                    (elab_st_typing d)
+                    (elab_comp c)) =
 
   let T_If _ b e1 e2  _ u_c hyp b_typing e1_typing e2_typing (E c_typing) = d in
   let rb_typing : RT.typing (extend_env_l f g)
-                            (elab_pure b)
+                            (elab_term b)
                             RT.bool_ty =
     tot_typing_soundness b_typing in
   let g_then = (hyp, Inl (mk_eq2 U_zero tm_bool b tm_true))::g in
@@ -358,10 +356,10 @@ let if_soundness
                                hyp
                                (RT.eq2 (R.pack_universe R.Uv_Zero)
                                        RT.bool_ty
-                                       (elab_pure b)
+                                       (elab_term b)
                                        RT.true_bool))
-                (elab_src_typing e1_typing)
-                (elab_pure_comp c) =
+                (elab_st_typing e1_typing)
+                (elab_comp c) =
     soundness f g_then e1 c e1_typing in
   let g_else = (hyp, Inl (mk_eq2 U_zero tm_bool b tm_false))::g in
   let re2_typing
@@ -369,112 +367,110 @@ let if_soundness
                                hyp
                                (RT.eq2 (R.pack_universe R.Uv_Zero)
                                        RT.bool_ty
-                                       (elab_pure b)
+                                       (elab_term b)
                                        RT.false_bool))
-                (elab_src_typing e2_typing)
-                (elab_pure_comp c) =
+                (elab_st_typing e2_typing)
+                (elab_comp c) =
     soundness f g_else e2 c e2_typing in
   let c_typing = 
     ct_soundness _ _ _ _ c_typing
   in
-  assume (~(hyp `Set.mem` RT.freevars (elab_src_typing e1_typing)));
-  assume (~(hyp `Set.mem` RT.freevars (elab_src_typing e2_typing)));  
+  assume (~(hyp `Set.mem` RT.freevars (elab_st_typing e1_typing)));
+  assume (~(hyp `Set.mem` RT.freevars (elab_st_typing e2_typing)));  
   RT.T_If _ _ _ _ _ _ _ rb_typing re1_typing re2_typing c_typing
 #pop-options
 
 #push-options "--query_stats --fuel 2 --ifuel 2 --z3rlimit_factor 10"
+
 let comp_typing_soundness (f:stt_env)
                           (g:env)
-                          (c:pure_comp)
+                          (c:comp)
                           (uc:universe)
                           (d:comp_typing f g c uc)
                           (soundness:soundness_t d)
-                          (tabs:tabs_t d)
-  : GTot (RT.typing (extend_env_l f g) (elab_pure_comp c) (RT.tm_type (elab_universe uc)))
+  : GTot (RT.typing (extend_env_l f g) (elab_comp c) (RT.tm_type (elab_universe uc)))
          (decreases d)
   = let stc_soundness (st:_) (d_st:st_comp_typing f g st { d_st << d }) 
-      : GTot (squash (Pulse.Elaborate.Pure.is_pure_st_comp st) &
-              RT.typing (extend_env_l f g) (elab_pure st.res) (RT.tm_type (elab_universe st.u)) &
-              RT.typing (extend_env_l f g) (elab_pure st.pre) vprop_tm &
-              RT.typing (extend_env_l f g) (mk_abs (elab_pure st.res) R.Q_Explicit
-                                                   (elab_pure st.post))
-                                           (post1_type_bind (elab_pure st.res)))
-      = let STC _ st x (E dres) (E dpre) (E dpost) = d_st in
-        let res_typing = soundness _ _ _ _ dres in
-        let pre_typing = soundness _ _ _ _ dpre in      
-        assert (elab_src_typing dpost == 
-                elab_pure (open_term st.post x));
+      : GTot (RT.typing (extend_env_l f g) (elab_term st.res) (RT.tm_type (elab_universe st.u)) &
+              RT.typing (extend_env_l f g) (elab_term st.pre) vprop_tm &
+              RT.typing (extend_env_l f g) (mk_abs (elab_term st.res) R.Q_Explicit
+                                                   (elab_term st.post))
+                                           (post1_type_bind (elab_term st.res)))
+      = let STC _ st x dres dpre dpost = d_st in
+        let res_typing = tot_typing_soundness dres in
+        let pre_typing = tot_typing_soundness dpre in      
         calc (==) {
-          RT.close_term (elab_pure (open_term st.post x)) x;
+          RT.close_term (elab_term (open_term st.post x)) x;
         (==) { elab_open_commute st.post x }
-          RT.close_term (RT.open_term (elab_pure st.post) x) x;
+          RT.close_term (RT.open_term (elab_term st.post) x) x;
         (==) { 
                elab_freevars_inverse st.post;
-               RT.close_open_inverse (elab_pure st.post) x
+               RT.close_open_inverse (elab_term st.post) x
              }
-          elab_pure st.post;
+          elab_term st.post;
         };
-        let post_typing  = tabs None RT.pp_name_default (E dres) dpost in
-        (), res_typing, pre_typing, post_typing
+        let post_typing  = mk_t_abs_tot f g RT.pp_name_default dres dpost in
+        res_typing, pre_typing, post_typing
     in
     match d with
-    | CT_Tot _ t _ (E dt) ->
-      soundness _ _ _ _ dt
+    | CT_Tot _ t _ dt ->
+      tot_typing_soundness dt
       
     | CT_ST _ st d_st -> 
-      let _, res_typing, pre_typing, post_typing = stc_soundness st d_st in
+      let res_typing, pre_typing, post_typing = stc_soundness st d_st in
       STT.stt_typing res_typing pre_typing post_typing
 
     | CT_STAtomic _ i st d_i d_st -> 
       let i_typing = tot_typing_soundness d_i in
-      let _, res_typing, pre_typing, post_typing = stc_soundness st d_st in
+      let res_typing, pre_typing, post_typing = stc_soundness st d_st in
       STT.stt_atomic_typing res_typing i_typing pre_typing post_typing
 
     | CT_STGhost _ i st d_i d_st -> 
       let i_typing = tot_typing_soundness d_i in
-      let _, res_typing, pre_typing, post_typing = stc_soundness st d_st in
+      let res_typing, pre_typing, post_typing = stc_soundness st d_st in
       STT.stt_ghost_typing res_typing i_typing pre_typing post_typing
 #pop-options
+
 #push-options "--query_stats --fuel 2 --ifuel 2"
 let rec soundness (f:stt_env)
                   (g:env)
-                  (t:term)
-                  (c:pure_comp)
-                  (d:src_typing f g t c)
-  : GTot (RT.typing (extend_env_l f g) (elab_src_typing d) (elab_pure_comp c))
+                  (t:st_term)
+                  (c:comp)
+                  (d:st_typing f g t c)
+  : GTot (RT.typing (extend_env_l f g) (elab_st_typing d) (elab_comp c))
          (decreases d)
   = let mk_t_abs (#f:stt_env)
                  (#g:env)
                  (#u:universe)
-                 (#ty:pure_term)
+                 (#ty:term)
                  (q:option qualifier)
                  (ppname:ppname)
                  (t_typing:tot_typing f g ty (Tm_Type u) { t_typing << d })
-                 (#body:term)
-                 (#x:var { None? (lookup g x) /\ ~(x `Set.mem` freevars body) })
-                 (#c:pure_comp)
-                 (body_typing:src_typing f ((x, Inl ty)::g) (open_term body x) c { body_typing << d })
+                 (#body:st_term)
+                 (#x:var { None? (lookup g x) /\ ~(x `Set.mem` freevars_st body) })
+                 (#c:comp)
+                 (body_typing:st_typing f ((x, Inl ty)::g) (open_st_term body x) c { body_typing << d })
       : GTot (RT.typing (extend_env_l f g)
-                        (mk_abs_with_name ppname (elab_pure ty) (elab_qual q) (RT.close_term (elab_src_typing body_typing) x))
-                        (elab_pure (Tm_Arrow {binder_ty=ty;binder_ppname=ppname} q (close_pure_comp c x))))
+                        (mk_abs_with_name ppname (elab_term ty) (elab_qual q) (RT.close_term (elab_st_typing body_typing) x))
+                        (elab_term (Tm_Arrow {binder_ty=ty;binder_ppname=ppname} q (close_comp c x))))
       = let E t_typing = t_typing in
-        let r_t_typing = soundness _ _ _ _ t_typing in
+        let r_t_typing = tot_typing_soundness (E t_typing) in
         let r_body_typing = soundness _ _ _ _ body_typing in
-        mk_t_abs f g ppname r_t_typing r_body_typing
+        mk_t_abs f g #_ #_ #_ #t_typing ppname r_t_typing r_body_typing
     in
-    LN.src_typing_ln d;
+    LN.st_typing_ln d;
     match d with
     | T_Lift _ _ _ _ _ _ ->
       lift_soundness _ _ _ _ d soundness
     | T_Frame _ _ _ _ _ _ ->
       frame_soundness _ _ _ _ d soundness
 
-    | T_Tot _ _ _ d -> d
+    | T_Tot _ _ _ d -> tot_typing_soundness d
 
-    | T_Abs _ ppname x q ty u body c t_typing body_typing ->
-      mk_t_abs q ppname t_typing body_typing    
+    | T_Abs _ x q ty u body c t_typing body_typing ->
+      mk_t_abs q RT.pp_name_default t_typing body_typing    
 
-    | T_STApp _ _ _ _ _ _ _ _ _ ->
+    | T_STApp _ _ _ _ _ _ _ _ ->
       stapp_soundness _ _ _ _ d soundness
 
     | T_Bind _ _e1 _e2 _c1 _c2 _x _c _e1_typing _t_typing _e2_typing _bc ->
@@ -492,7 +488,7 @@ let rec soundness (f:stt_env)
 
     | T_If _ _ _ _ _ _ _ _ _ _ _->
       let ct_soundness f g c uc (d':_ {d' << d}) =
-        comp_typing_soundness f g c uc d' soundness mk_t_abs
+        comp_typing_soundness f g c uc d' soundness
       in
       if_soundness _ _ _ _ d soundness ct_soundness
 
@@ -508,13 +504,13 @@ let rec soundness (f:stt_env)
 let soundness_lemma
   (f:stt_env)
   (g:env)
-  (t:term)
-  (c:pure_comp)
-  (d:src_typing f g t c)
+  (t:st_term)
+  (c:comp)
+  (d:st_typing f g t c)
   : Lemma (ensures RT.typing (extend_env_l f g)
-                             (elab_src_typing d)
-                             (elab_pure_comp c))
+                             (elab_st_typing d)
+                             (elab_comp c))
   = FStar.Squash.bind_squash
-      #(src_typing f g t c)
+      #(st_typing f g t c)
       ()
       (fun dd -> FStar.Squash.return_squash (soundness f g t c d))
